WIP use rcond, wcond and zcond -- draft for FTRL store

theories/ftlr/Store.v
@@ -30,59 +30,183 @@ Section fundamental.
 
   (* The necessary resources to close the region again,
       except for the points to predicate, which we will store separately *)
-  Definition region_open_resources W l ls p φ (v : Word): iProp Σ :=
-    (∃ ρ,
-        sts_state_std l ρ
-        ∗ ⌜std W !! l = Some ρ⌝
-        ∗ ⌜ρ ≠ Revoked⌝
-        ∗ ⌜(∀ g, ρ ≠ Frozen g)⌝
-        ∗ open_region_many (l :: ls) W
-        ∗ rel l p φ)%I.
+  (* Definition region_open_resources W l ls p φ (v : Word): iProp Σ := *)
+  (*   (∃ ρ, *)
+  (*       sts_state_std l ρ *)
+  (*       ∗ ⌜std W !! l = Some ρ⌝ *)
+  (*       ∗ ⌜ρ ≠ Revoked⌝ *)
+  (*       ∗ ⌜(∀ g, ρ ≠ Frozen g)⌝ *)
+  (*       ∗ open_region_many (l :: ls) W *)
+  (*       ∗ rel l p φ)%I. *)
 
-  Lemma store_inr_eq {regs r p0 g0 b0 e0 a0 p1 g1 b1 e1 a1 storev}:
-    reg_allows_store regs r p0 g0 b0 e0 a0 storev →
-    read_reg_inr regs r p1 g1 b1 e1 a1 →
-    p0 = p1 ∧ g0 = g1 ∧ b0 = b1 ∧ e0 = e1 ∧ a0 = a1.
+
+  Definition later_zcond (P : D) (has_later : bool) :=
+    if has_later
+    then (▷ □ ∀ W1 W2 (z : Z), P W1 (WInt z) -∗ P W2 (WInt z))%I
+    else (□ ∀ W1 W2 (z : Z), P W1 (WInt z) -∗ P W2 (WInt z))%I.
+
+  Definition later_wcond (P : D) (has_later : bool) :=
+    if has_later
+    then ( ▷ □ ∀ W (w : Word), interp W w -∗ P W w)%I
+    else ( □ ∀ W (w : Word), interp W w -∗ P W w)%I.
+
+  Definition later_rcond (P : D) (has_later : bool):=
+    if has_later
+    then ( ▷ □ ∀ W (w : Word), P W w -∗ interp W w)%I
+    else ( □ ∀ W (w : Word), P W w -∗ interp W w)%I.
+
+  Lemma P_zcond_monotone_generalZ
+    (W : WORLD) (ρ : region_type) (p : Perm) (a : Addr) (z : Z) (P : D) :
+    std W !! a = Some ρ →
+    later_zcond P false -∗
+    monotonicity_guarantees_region ρ (WInt z) p (λ Wv : WORLD * (leibnizO Word), (P Wv.1) Wv.2).
   Proof.
-    intros Hrar H3.
-    pose (Hrar' := Hrar).
-    destruct Hrar' as (Hinr0 & _). rewrite /read_reg_inr Hinr0 in H3.
-    by inversion H3.
+    unfold monotonicity_guarantees_region.
+    iIntros (Hstd) "#Hzcond".
+    destruct ρ;auto.
+    - destruct (pwl p) eqn: HpwlP1 ; iModIntro; simpl; iIntros (W0 W1) "% HIW0".
+      all: by iApply "Hzcond".
+    - iModIntro; simpl; iIntros (W0 W1) "% HIW0".
+      by iApply "Hzcond".
   Qed.
 
-  (* Description of what the resources are supposed to look like
-     after opening the region if we need to,
-     but before closing the region up again*)
-  Definition allow_store_res W r1 r2 (regs : Reg) pc_a (pc_p : Perm) :=
-    (∃ p g b e a storev,
-        ⌜read_reg_inr regs r1 p g b e a⌝
-        ∗ ⌜word_of_argument regs r2 = Some storev⌝
-        ∗ if decide (reg_allows_store regs r1 p g b e a storev )
-          then (if decide (a ≠ pc_a)
-                then ∃ p' (P':D) w,
-                    ⌜PermFlows p p'⌝
-                    ∗ ⌜ persistent_cond P' ⌝
-                    ∗ a ↦ₐ w
-                    ∗ (region_open_resources W a [pc_a] p'
-                         (λ Wv : WORLD * (leibnizO Word), (P' Wv.1) Wv.2) w)
-                else open_region pc_a W ∗ ⌜PermFlows p pc_p⌝  )
-          else open_region pc_a W)%I.
+Lemma P_monotone_generalSd (W : WORLD) (ρ : region_type)
+  (p p' : Perm) (g : Locality) (b e a : Addr)
+  (ot : OType) (sb : Sealable) (P : D) :
+  std W !! a = Some ρ →
+  withinBounds b e a = true →
+  PermFlows p p' →
+  ((fixpoint interp1) W) (WCap p g b e a)
+  -∗ ((fixpoint interp1) W) (WSealed ot sb)
+  -∗ later_wcond P false
+  -∗ monotonicity_guarantees_region ρ (WSealed ot sb) p' (λ Wv : WORLD * (leibnizO Word), (P Wv.1) Wv.2).
+Proof.
+  unfold monotonicity_guarantees_region.
+  iIntros (Hstd Hwb Hfl') "#Hvdst #Hvsrc #Hwcond".
+  destruct ρ;auto.
+  - destruct (pwl p') eqn: Hpwlp' ; iModIntro; simpl; iIntros (W0 W1) "% HIW0".
+    + iApply "Hwcond"; rewrite !fixpoint_interp1_eq; iEval (cbn) in "Hvsrc"; iEval (cbn); done.
+    + iApply "Hwcond"; rewrite !fixpoint_interp1_eq; iEval (cbn) in "Hvsrc"; iEval (cbn); done.
+  - iModIntro; simpl; iIntros (W0 W1) "% HIW0".
+    iApply "Hwcond"; rewrite !fixpoint_interp1_eq; iEval (cbn) in "Hvsrc"; iEval (cbn); done.
+Qed.
+
+Lemma P_monotone_generalSr (W : WORLD) (ρ : region_type)
+  (p p' : Perm) (g : Locality) (b e a : Addr)
+  (sp : SealPerms) (sg : Locality) (sb se sa : OType) (P:D) :
+  std W !! a = Some ρ →
+  withinBounds b e a = true →
+  PermFlows p p' →
+  ((fixpoint interp1) W) (WCap p g b e a)
+  -∗ ((fixpoint interp1) W) (WSealRange sp sg sb se sa)
+  -∗ later_wcond P false
+  -∗ monotonicity_guarantees_region ρ (WSealRange sp sg sb se sa) p' (λ Wv : WORLD * (leibnizO Word), (P Wv.1) Wv.2).
+Proof.
+  unfold monotonicity_guarantees_region.
+  iIntros (Hstd Hwb Hfl') "#Hvdst #Hvsrc #Hwcond".
+  destruct ρ;auto.
+  - destruct (pwl p') eqn: Hpwlp' ; iModIntro; simpl; iIntros (W0 W1) "% HIW0".
+    + iApply "Hwcond"; rewrite !fixpoint_interp1_eq; iEval (cbn) in "Hvsrc"; iEval (cbn); done.
+    + iApply "Hwcond"; rewrite !fixpoint_interp1_eq; iEval (cbn) in "Hvsrc"; iEval (cbn); done.
+  - iModIntro; simpl; iIntros (W0 W1) "% HIW0".
+    iApply "Hwcond"; rewrite !fixpoint_interp1_eq; iEval (cbn) in "Hvsrc"; iEval (cbn); done.
+Qed.
+
+Lemma P_monotone_generalW (W : WORLD)  (ρ : region_type)
+  (p p' p'' : Perm) (g g' : Locality) (b e a b' e' a' : Addr) (P:D) :
+  std W !! a' = Some ρ →
+  withinBounds b' e' a' = true →
+  PermFlows p' p'' →
+  canStore p' (WCap p g b e a) = true →
+  ((fixpoint interp1) W) (WCap p' g' b' e' a')
+  -∗ ((fixpoint interp1) W) (WCap p g b e a)
+  -∗ later_wcond P false
+  -∗ monotonicity_guarantees_region ρ (WCap p g b e a) p''
+    (λ Wv : WORLD * (leibnizO Word), (P Wv.1) Wv.2).
+Proof.
+  unfold monotonicity_guarantees_region.
+  iIntros (Hstd Hwb Hfl' Hconds) "#Hvdst #Hvsrc #Hwcond".
+  destruct ρ;simpl;auto.
+  - destruct (pwl p'') eqn: HpwlP'' ; iModIntro; simpl;auto; iIntros (W0 W1) "% HIW0".
+    * iApply "Hwcond".
+      iApply interp_monotone; eauto.
+    * destruct g; first by iApply interp_monotone_nl.
+    (* The below case is a contradiction, since if g is local,
+      p' must be WL and p' flows into the non-WL p''*)
+      destruct p' ; try (simpl in Hconds; by exfalso).
+      all:destruct p'' eqn:Hp''v ; (by exfalso).
+  - iModIntro; iIntros (W0 W1) "% HIW0".
+    destruct g.
+    + by iApply interp_monotone_nl.
+    + (*Trick here: value relation leads to a contradiction if p' is WL,
+        since then its region cannot be permanent *)
+      iDestruct ( writeLocalAllowed_valid_cap_implies with "Hvdst" ) as %Ha; eauto.
+      by rewrite Hstd in Ha.
+Qed.
+
+  Lemma monotonicity_guarantees_wf (P : D) ρ w p :
+    later_rcond P false
+    -∗ later_wcond P false
+       -∗ monotonicity_guarantees_region
+            ρ w p (λ Wv : WORLD * (leibnizO Word), (interp Wv.1) Wv.2)
+          -∗ monotonicity_guarantees_region
+               ρ w p (λ Wv : WORLD * (leibnizO Word), (P Wv.1) Wv.2).
+  Proof.
+    iIntros "#Hrcond #Hwcond HmonoV"; cbn.
+    rewrite /monotonicity_guarantees_region.
+    destruct ρ; auto.
+    destruct (pwl p); auto; iDestruct "HmonoV" as "#HmonoV".
+    - iModIntro. iIntros (W0 W1 Hrelated) "HP".
+      iApply "Hwcond".
+      iApply "HmonoV"; auto.
+      iApply "Hrcond".
+      done.
+    - iModIntro. iIntros (W0 W1 Hrelated) "HP".
+      iApply "Hwcond".
+      iApply "HmonoV"; auto.
+      iApply "Hrcond".
+      done.
+    - iDestruct "HmonoV" as "#HmonoV".
+      iModIntro. iIntros (W0 W1 Hrelated) "HP".
+      iApply "Hwcond".
+      iApply "HmonoV"; auto.
+      iApply "Hrcond".
+      done.
+    Qed.
 
 
-  Definition allow_store_mem W r1 r2 (regs : Reg) pc_a (pc_p : Perm) pc_w (mem : Mem) :=
-    (∃ p g b e a storev, ⌜read_reg_inr regs r1 p g b e a⌝
-                         ∗ ⌜word_of_argument regs r2 = Some storev⌝
-                         ∗ if decide (reg_allows_store regs r1 p g b e a storev)
-                           then (if decide (a ≠ pc_a)
-                                 then ∃ p' (P':D) w,
-                                     ⌜PermFlows p p'⌝
-                                     ∗ ⌜ persistent_cond P' ⌝
-                                     ∗ ⌜mem = <[a:=w]> (<[pc_a:=pc_w]> ∅)⌝
-                                     ∗ (region_open_resources W a [pc_a] p'
-                                          (λ Wv : WORLD * (leibnizO Word), (P' Wv.1) Wv.2)
-                                          w)
-                                 else  ⌜mem = <[pc_a:=pc_w]> ∅⌝ ∗ open_region pc_a W  ∗ ⌜PermFlows p pc_p⌝)
-                           else  ⌜mem = <[pc_a:=pc_w]> ∅⌝ ∗ open_region pc_a W)%I.
+  (* Lemma storev_P_mono W (r : Reg) (r1 : RegName) (r2 : Z + RegName) p g b e a p' ρ storev: *)
+  (*    PermFlows p p' *)
+  (*   -> word_of_argument r r2 = Some storev *)
+  (*   → reg_allows_store r r1 p g b e a storev *)
+  (*   → std W !! a = Some ρ *)
+  (*   → (fixpoint interp1) W (WCap p g b e a) *)
+  (*   (* -∗ (fixpoint interp1) W storev *) *)
+  (*   (* -∗ later_zcond P false *) *)
+  (*   (* -∗ (if writeAllowed p' then later_wcond P false else True) *) *)
+  (*   (* -∗ (if readAllowed p' then later_rcond P false else True) *) *)
+  (*   -∗ ∃ (P:D), *)
+  (*       ⌜persistent_cond P⌝ *)
+  (*       ∗ zcond P *)
+  (*       ∗ rcond P interp *)
+  (*       ∗ wcond P interp *)
+  (*       ∗ monotonicity_guarantees_region ρ storev p' *)
+  (*        (λ Wv : WORLD * (leibnizO Word), (P Wv.1) Wv.2). *)
+  (* Proof. *)
+  (*   iIntros (Hflp Hwoa Hras Hststd) "HInt". *)
+  (*   destruct Hras as (Hrir & Hwa & Hwb & Hloc). *)
+  (*   rewrite /monotonicity_guarantees_region. *)
+  (*   destruct storev as [z | sb | ot sb ]. *)
+  (*   (* - iApply (P_zcond_monotone_generalZ with "[HInt]" ); eauto. *) *)
+  (*   (* - admit. *) *)
+  (*   (* - rewrite /monotonicity_guarantees_region. *) *)
+  (*   (*   destruct ρ;auto. *) *)
+  (*   (*   2: { iModIntro; simpl; iIntros (W0 W1) "% HIW0". *) *)
+  (*   (*        replace (writeAllowed p') with true; last admit. *) *)
+  (*   (*        iApply "Hwcond". *) *)
+  (*   (*        admit. *) *)
+  (*   (*   } *) *)
+  (* Abort. *)
 
   Lemma interp_hpf_eq (W : WORLD) P (regs : leibnizO Reg) (r1 : RegName)
     p g b e a pc_p pc_g pc_b pc_e pc_p' w storev:
@@ -107,6 +231,111 @@ Section fundamental.
       done.
   Qed.
 
+  Lemma storev_interp_mono W (r : Reg) (r1 : RegName) (r2 : Z + RegName) p g b e a p' ρ storev:
+     PermFlows p p'
+    -> word_of_argument r r2 = Some storev
+    → reg_allows_store r r1 p g b e a storev
+    → std W !! a = Some ρ
+    → ((fixpoint interp1) W) (WCap p g b e a)
+    -∗ monotonicity_guarantees_region ρ storev p'
+         (λ Wv : WORLD * (leibnizO Word), (interp Wv.1) Wv.2).
+  Proof.
+    iIntros (Hflp Hwoa Hras Hststd) "HInt".
+    destruct Hras as (Hrir & Hwa & Hwb & Hloc).
+    destruct storev as [z | sb | ot sb ].
+    - iApply (interp_monotone_generalZ with "[HInt]" ); eauto.
+    - destruct sb ;
+        [ iApply (interp_monotone_generalW with "[HInt]" )
+        | iApply (interp_monotone_generalSr with "[HInt]" )]
+      ; eauto.
+    - iApply (interp_monotone_generalSd with "[HInt]" ); eauto.
+  Qed.
+
+  Lemma storev_P_mono W P (r : Reg) (r1 : RegName) (r2 : Z + RegName) p g b e a p' ρ storev:
+     PermFlows p p'
+    -> word_of_argument r r2 = Some storev
+    → reg_allows_store r r1 p g b e a storev
+    → std W !! a = Some ρ
+    → ((fixpoint interp1) W) (WCap p g b e a)
+    -∗ later_rcond P false
+    -∗ later_wcond P false
+    -∗ monotonicity_guarantees_region ρ storev p'
+         (λ Wv : WORLD * (leibnizO Word), (P Wv.1) Wv.2).
+  Proof.
+    iIntros (Hflp Hwoa Hras Hststd) "#HInt #Hrcond #Hwcond".
+    iAssert
+     (monotonicity_guarantees_region ρ storev p'
+         (λ Wv : WORLD * (leibnizO Word), (interp Wv.1) Wv.2)) as "HmonoV".
+    { iApply storev_interp_mono ; eauto. }
+    iApply monotonicity_guarantees_wf; eauto.
+  Qed.
+
+
+  Definition region_open_resources W l ls p φ (v : Word): iProp Σ :=
+    (∃ ρ,
+        sts_state_std l ρ
+        ∗ ⌜std W !! l = Some ρ⌝
+        ∗ ⌜ρ ≠ Revoked⌝
+        ∗ ⌜(∀ g, ρ ≠ Frozen g)⌝
+        ∗ open_region_many (l :: ls) W
+        ∗ rel l p φ)%I.
+
+  Lemma store_inr_eq {regs r p0 g0 b0 e0 a0 p1 g1 b1 e1 a1 storev}:
+    reg_allows_store regs r p0 g0 b0 e0 a0 storev →
+    read_reg_inr regs r p1 g1 b1 e1 a1 →
+    p0 = p1 ∧ g0 = g1 ∧ b0 = b1 ∧ e0 = e1 ∧ a0 = a1.
+  Proof.
+    intros Hrar H3.
+    pose (Hrar' := Hrar).
+    destruct Hrar' as (Hinr0 & _). rewrite /read_reg_inr Hinr0 in H3.
+    by inversion H3.
+  Qed.
+
+  (* Lemma later_wcond_later_is_wcond (P:D) : *)
+  (*   later_wcond true P ∗-∗ wcond P interp. *)
+  (* Proof. *)
+  (*   iSplit; iIntros ; cbn ; done. *)
+  (* Qed. *)
+
+  (* Description of what the resources are supposed to look like
+     after opening the region if we need to,
+     but before closing the region up again*)
+  Definition allow_store_res W r1 r2 (regs : Reg) pc_a (pc_p : Perm) (has_later : bool) :=
+    (∃ p g b e a storev,
+        ⌜read_reg_inr regs r1 p g b e a⌝
+        ∗ ⌜word_of_argument regs r2 = Some storev⌝
+        ∗ if decide (reg_allows_store regs r1 p g b e a storev )
+          then (if decide (a ≠ pc_a)
+                then ∃ p' (P':D) w,
+                    ⌜PermFlows p p'⌝
+                    ∗ ⌜ persistent_cond P' ⌝
+                    ∗ a ↦ₐ w
+                    ∗ later_zcond P' has_later
+                    ∗ (if writeAllowed p' then later_wcond P' has_later else True)
+                    ∗ (if readAllowed p' then later_rcond P' has_later else True)
+                    ∗ (region_open_resources W a [pc_a] p'
+                         (λ Wv : WORLD * (leibnizO Word), (P' Wv.1) Wv.2) w)
+                else open_region pc_a W ∗ ⌜PermFlows p pc_p⌝  )
+          else open_region pc_a W)%I.
+
+  Definition allow_store_mem W r1 r2 (regs : Reg) pc_a (pc_p : Perm) pc_w (mem : Mem)
+    (has_later : bool) :=
+    (∃ p g b e a storev, ⌜read_reg_inr regs r1 p g b e a⌝
+                         ∗ ⌜word_of_argument regs r2 = Some storev⌝
+                         ∗ if decide (reg_allows_store regs r1 p g b e a storev)
+                           then (if decide (a ≠ pc_a)
+                                 then ∃ p' (P':D) w,
+                                     ⌜PermFlows p p'⌝
+                                     ∗ ⌜ persistent_cond P' ⌝
+                                     ∗ later_zcond P' has_later
+                                     ∗ (if writeAllowed p' then later_wcond P' has_later else True)
+                                     ∗ (if readAllowed p' then later_rcond P' has_later else True)
+                                     ∗ ⌜mem = <[a:=w]> (<[pc_a:=pc_w]> ∅)⌝
+                                     ∗ (region_open_resources W a [pc_a] p'
+                                          (λ Wv : WORLD * (leibnizO Word), (P' Wv.1) Wv.2) w )
+                                 else  ⌜mem = <[pc_a:=pc_w]> ∅⌝ ∗ open_region pc_a W  ∗ ⌜PermFlows p pc_p⌝)
+                           else  ⌜mem = <[pc_a:=pc_w]> ∅⌝ ∗ open_region pc_a W)%I.
+
   Lemma create_store_res:
     ∀ (W : WORLD) (regs : leibnizO Reg)
       (p p' : Perm) (g : Locality) (b e a : Addr)
@@ -120,7 +349,7 @@ Section fundamental.
     -∗ rel a p' (λ Wv : STS_std_states Addr region_type * (STS_states * STS_rels) * Word, P Wv.1 Wv.2)
     -∗ open_region a W
     -∗ sts_full_world W
-    -∗ allow_store_res W r1 r2 (<[PC:=WCap p g b e a]> regs) a p'
+    -∗ allow_store_res W r1 r2 (<[PC:=WCap p g b e a]> regs) a p' true
     ∗ sts_full_world W.
   Proof.
     intros W regs p p' g b e a r1 r2 p0 g0 b0 e0 a0 storev P HVr1 Hfl Hwoa.
@@ -145,17 +374,23 @@ Section fundamental.
       iDestruct (readAllowed_valid_cap_implies with "Hvsrc") as %HH; eauto.
       { by apply writeA_implies_readA. }
       { rewrite /withinBounds Hge; solve_addr. }
+
+      rewrite Hra; simpl.
       destruct HH as [ρ' [Hstd' [Hnotrevoked' Hnotfrozen'] ] ].
       (* We can finally frame off Hsts here, since it is no longer needed after opening the region*)
-      rewrite Hra.
       iDestruct (region_open_next _ _ _ a0 p'' ρ' with "[$Hrel'' $Hr $Hsts]")
         as (w0) "($ & Hstate' & Hr & Ha0 & Hfuture & Hval)"; eauto.
       { intros [g1 Hcontr];specialize (Hnotfrozen' g1); contradiction. }
       { apply not_elem_of_cons. split; auto. apply not_elem_of_nil. }
       iExists p'',P''.
+      iAssert ((if writeAllowed p'' then later_wcond P'' true else True)%I) as "Hwcond'".
+      { destruct (writeAllowed p''); done. }
+      iAssert ((if readAllowed p'' then later_rcond P'' true else True)%I) as "Hrcond'".
+      { destruct (readAllowed p''); done. }
+
       iFrame "∗#".
       iSplitR;[iPureIntro ; destruct p0,p'; done|].
-      iSplitR; iPureIntro;done.
+      iSplitR; try (iPureIntro; done).
     - simplify_eq; iFrame.
       iApply interp_hpf_eq; eauto.
   Qed.
@@ -163,10 +398,11 @@ Section fundamental.
   Lemma store_res_implies_mem_map:
     ∀ (W : WORLD) (regs : leibnizO Reg)
       (p' : Perm) (a : Addr) (w : Word) (r1 : RegName) (r2 : Z + RegName),
-    allow_store_res W r1 r2 regs a p'
+    allow_store_res W r1 r2 regs a p' true
     -∗ a ↦ₐ w
     -∗ ∃ mem0 : Mem,
-        allow_store_mem W r1 r2 regs a p' w mem0 ∗ ▷ ([∗ map] a0↦w0 ∈ mem0, a0 ↦ₐ w0).
+        allow_store_mem W r1 r2 regs a p' w mem0 true
+        ∗ ▷ ([∗ map] a0↦w0 ∈ mem0, a0 ↦ₐ w0).
   Proof.
     intros W regs p' a w r1 r2.
     iIntros "HStoreRes Ha".
@@ -174,13 +410,14 @@ Section fundamental.
     case_decide as Hallows.
     - case_decide as Haeq.
       + pose(Hallows' := Hallows). destruct Hallows as (Hrinr & Hra & Hwb & HLoc).
-        iDestruct "HStoreRes" as (p0' P0' w0 Hflp' HpersP0') "[HStoreCh HStoreRest]".
+        iDestruct "HStoreRes" as (p0' P0' w0 Hflp' HpersP0')
+                                   "(HStoreCh & #Hzcond & #Hwcond & #Hrcond & HStoreRest)".
         iExists _.
         iSplitL "HStoreRest".
         ++ iExists p1,g1,b1,e1,a1,storev. iFrame "%".
            case_decide; last by exfalso. case_decide; last by exfalso.
            iExists p0',P0',w0.
-           iSplitR; auto.
+           repeat (iSplitR; auto).
         ++ iNext; iApply memMap_resource_2ne; auto; iFrame.
       + iExists _.
         iSplitL "HStoreRes"; last (iNext; by iApply memMap_resource_1).
@@ -198,7 +435,7 @@ Section fundamental.
       (p p' : Perm) (g : Locality) (b e a : Addr)
       (w : Word) (r1 : RegName) (r2 : Z + RegName)
       (mem0 : Mem),
-    allow_store_mem W r1 r2 regs a p' w mem0
+    allow_store_mem W r1 r2 regs a p' w mem0 true
     -∗ ⌜mem0 !! a = Some w⌝
     ∗ ⌜allow_store_map_or_true r1 r2 regs mem0⌝.
   Proof.
@@ -207,7 +444,7 @@ Section fundamental.
     case_decide as Hallows.
     - case_decide as Haeq.
       + pose(Hallows' := Hallows). destruct Hallows' as (Hrinr & Hra & Hwb & HLoc).
-        iDestruct "HStoreRes" as (p0' P0' w0 Hflp' HpersP0') "[% _]".
+        iDestruct "HStoreRes" as (p0' P0' w0 Hflp' HpersP0') "(_ & _ & _ & % & _)".
         iSplitR. subst. rewrite lookup_insert_ne; auto. by rewrite lookup_insert.
         iExists p1,g1,b1,e1,a1,storev.
         iPureIntro. repeat split; auto.
@@ -224,29 +461,11 @@ Section fundamental.
       case_decide as Hdec1; last by done. by exfalso.
   Qed.
 
-  Lemma storev_interp_mono W (r : Reg) (r1 : RegName) (r2 : Z + RegName) p g b e a p' P ρ storev:
-     PermFlows p p'
-    -> word_of_argument r r2 = Some storev
-    → reg_allows_store r r1 p g b e a storev
-    → std W !! a = Some ρ
-    → ((fixpoint interp1) W) (WCap p g b e a)
-    -∗ rel a p' (λ Wv : WORLD * leibnizO Word, P Wv.1 Wv.2)
-    -∗ monotonicity_guarantees_region ρ storev p'
-         (λ Wv : WORLD * (leibnizO Word), (P Wv.1) Wv.2).
-  Proof.
-    iIntros (Hflp Hwoa Hras Hststd) "HInt".
-    (* iExists interp. *)
-    (* destruct Hras as (Hrir & Hwa & Hwb & Hloc). *)
-    (* destruct storev as [z | sb | ot sb ]. *)
-    (* - iApply (interp_monotone_generalZ with "[HInt]" ); eauto. *)
-    (* - destruct sb ; *)
-    (*     [ iApply (interp_monotone_generalW with "[HInt]" ) *)
-    (*     | iApply (interp_monotone_generalSr with "[HInt]" )] *)
-    (*   ; eauto. *)
-    (* - iApply (interp_monotone_generalSd with "[HInt]" ); eauto. *)
-  Admitted.
 
-  Definition wcond' (P : D) p g b e a r : iProp Σ := (if decide (writeAllowed_in_r_a (<[PC:= WCap p g b e a]> r) a) then □ (∀ W0 (w : Word), interp W0 w -∗ P W0 w) else emp)%I.
+  Definition wcond' (P : D) p g b e a r : iProp Σ
+    := (if decide (writeAllowed_in_r_a (<[PC:= WCap p g b e a]> r) a)
+        then □ (∀ W0 (w : Word), interp W0 w -∗ P W0 w)
+        else emp)%I.
   Instance wcond'_pers P p g b e a r: Persistent (wcond' P p g b e a r).
   Proof. intros. rewrite /wcond'. case_decide;apply _. Qed.
 
@@ -260,11 +479,11 @@ Section fundamental.
     → reg_allows_store (<[PC:= WCap pc_p pc_g pc_b pc_e pc_a]> regs) r1 p0 g0 b0 e0 a0 storev
     → std W !! pc_a = Some ρ
     → mem0 !! a0 = Some oldv (*?*)
-    → allow_store_mem W r1 r2 (<[PC:=WCap pc_p pc_g pc_b pc_e pc_a]> regs) pc_a pc_p'  pc_w mem0
+    → allow_store_mem W r1 r2 (<[PC:=WCap pc_p pc_g pc_b pc_e pc_a]> regs) pc_a pc_p'  pc_w mem0 false
     -∗ (∀ (r1 : RegName) v, ⌜r1 ≠ PC⌝ → ⌜regs !! r1 = Some v⌝ → ((fixpoint interp1) W) v)
     -∗ ((fixpoint interp1) W) (WCap pc_p pc_g pc_b pc_e pc_a)
     -∗ P W pc_w
-    -∗ □ (∀ W0 (w : Word), P W0 w -∗ interp W0 w)
+    -∗ later_rcond P false
     -∗ wcond' P pc_p pc_g pc_b pc_e pc_a regs
     -∗ monotonicity_guarantees_region ρ pc_w pc_p' (λ Wv : WORLD * Word, P Wv.1 Wv.2)
     -∗ ([∗ map] a0↦w0 ∈ <[a0 := storev]> mem0, a0 ↦ₐ w0)
@@ -275,79 +494,112 @@ Section fundamental.
     iDestruct "HStoreMem" as (p1 g1 b1 e1 a1 storev1) "[% [% HStoreRes] ]".
     destruct (store_inr_eq Hras H) as (<- & <- &<- &<- &<-).
     inversion H0; simplify_eq.
-    case_decide as Hallows.
-    - iAssert (((fixpoint interp1) W) (WCap p0 g0 b0 e0 a0))%I with "[HVPCr Hreg]" as "#HVr1".
-      { destruct Hras as [Hreg _]. destruct (decide (r1 = PC)).
-        - subst r1. rewrite lookup_insert in Hreg; by inversion Hreg.
-        - simplify_map_eq.
-          by iSpecialize ("Hreg" $! r1 _ n Hreg).
-      }
-      iAssert (((fixpoint interp1) W) storev)%I with "[HVPCr Hreg]" as "#HVstorev1".
-      { destruct storev.
-        - repeat rewrite fixpoint_interp1_eq. by cbn.
-        - destruct r2. cbn in Hwoa; inversion Hwoa; by exfalso.
-          cbn in Hwoa.
-          destruct (decide (r = PC)).
-          + subst r. simplify_map_eq. done.
-          + simplify_map_eq.
-            iSpecialize ("Hreg" $! r _ n Hwoa).
-            done.
-        - destruct r2. cbn in Hwoa; inversion Hwoa; by exfalso.
-          cbn in Hwoa.
-          destruct (decide (r = PC)).
-          + subst r. simplify_map_eq.
-          + simplify_map_eq.
-            iSpecialize ("Hreg" $! r _ n Hwoa).
-            done.
-      }
-      case_decide as Haeq.
-      + iExists pc_w.
-        destruct Hallows as [Hrinr [Hwa [Hwb Hloc] ] ].
-        iDestruct "HStoreRes" as (p' P' w' Hflp' HpersP') "[-> HLoadRes]".
-        rewrite lookup_insert in Ha0; inversion Ha0; clear Ha0; subst.
-        iDestruct "HLoadRes" as (ρ1) "(Hstate' & % & % & % & Hr & #Hrel')".
-        rewrite insert_insert memMap_resource_2ne; last auto. iDestruct "Hmem" as  "[Ha1 $]".
-        (* iFrame. *)
-        iDestruct (storev_interp_mono with "[$HVr1] [Hrel']") as "Hr1Mono"; eauto.
-        admit.
-        iDestruct (region_close_next with "[$Hr $Ha1 $Hrel' $Hstate' HVstorev1 Hr1Mono]") as "Hr"; eauto.
-        { intros [g Hcontr]. specialize (H2 g). done. }
-        { apply not_elem_of_cons; split; [auto|apply not_elem_of_nil]. }
-        { iSplit.
-          iPureIntro ; clear -Hflp' Hwa; destruct p0,p'; cbn in *; try done.
-          iSplitL. admit. (* TODO Just Rocq typechecking  *)
-          admit.
-          (* TODO I should be able to derive ▷(P' ≡ interp) at some point in the proof. *)
-        }
-        iDestruct (region_open_prepare with "Hr") as "$". iFrame.
-      + subst a0. iDestruct "HStoreRes" as "[-> [HStoreRes %]]".
-        rewrite insert_insert -memMap_resource_1.
-        rewrite lookup_insert in Ha0; inversion Ha0; simplify_eq.
-        iExists storev. iFrame. rewrite /wcond'.
-        admit.
-        (* rewrite decide_True. *)
-        (* iSplitR;[iApply "Hwcond";iFrame "#"|]. *)
-        (* iDestruct (storev_interp_mono with "HVr1") as "Hr1Mono"; eauto. *)
-        (* rewrite /monotonicity_guarantees_region. *)
-        (* destruct ρ;auto. *)
-        (* { destruct (pwl pc_p'); iModIntro; iIntros (W1 W2 Hrelated) "H". *)
-        (*   all:iApply "Hwcond"; iApply "Hr1Mono"; eauto; iApply "Hrcond"; iFrame. *)
-        (* } *)
-        (* { destruct (pwl pc_p'); iModIntro; iIntros (W1 W2 Hrelated) "H". *)
-        (*   all:iApply "Hwcond"; iApply "Hr1Mono"; eauto; iApply "Hrcond"; iFrame. *)
-        (* } *)
-        (* rewrite /writeAllowed_in_r_a. eexists r1, _. inversion Hras. *)
-        (* split. eassumption. *)
-        (* destruct H1. destruct H2. *)
-        (* split;auto. *)
-        (* split;auto. *)
-        (* destruct H2. *)
-        (* apply withinBounds_le_addr in H2; auto. *)
-    - by exfalso.
-   Admitted.
+    case_decide as Hallows; last by exfalso.
+    iAssert (((fixpoint interp1) W) (WCap p0 g0 b0 e0 a0))%I with "[HVPCr Hreg]" as "#HVr1".
+    { destruct Hras as [Hreg _]. destruct (decide (r1 = PC)).
+      - subst r1. rewrite lookup_insert in Hreg; by inversion Hreg.
+      - simplify_map_eq.
+        by iSpecialize ("Hreg" $! r1 _ n Hreg).
+    }
+    iAssert (((fixpoint interp1) W) storev)%I with "[HVPCr Hreg]" as "#HVstorev1".
+    { destruct storev.
+      - iEval (rewrite fixpoint_interp1_eq); by cbn.
+      - destruct r2. cbn in Hwoa; inversion Hwoa; by exfalso.
+        cbn in Hwoa.
+        destruct (decide (r = PC)).
+        + subst r; simplify_map_eq. done.
+        + simplify_map_eq.
+          iSpecialize ("Hreg" $! r _ n Hwoa).
+          done.
+      - destruct r2. cbn in Hwoa; inversion Hwoa; by exfalso.
+        cbn in Hwoa.
+        destruct (decide (r = PC)).
+        + subst r; simplify_map_eq.
+        + simplify_map_eq.
+          iSpecialize ("Hreg" $! r _ n Hwoa).
+          done.
+    }
+    case_decide as Haeq.
+    + iExists pc_w.
+      destruct Hallows as [Hrinr [Hwa [Hwb Hloc] ] ].
+      iDestruct "HStoreRes" as (p' P' w' Hflp' HpersP') "(#Hzcond' & #Hwcond' & #Hrcond' & -> & HLoadRes)".
+      rewrite lookup_insert in Ha0; inversion Ha0; clear Ha0; subst.
+      iDestruct "HLoadRes" as (ρ1) "(Hstate' & % & % & % & Hr & #Hrel')".
 
-   Lemma if_later {C} {eqdec: Decision C} (P:D) interp (Q Q' : iProp Σ) : (if (decide C) then ▷ Q else Q') -∗ ▷ (if (decide C) then Q else Q').
+      rewrite insert_insert memMap_resource_2ne; last auto.
+      iDestruct "Hmem" as  "[Ha1 Hpc_a]".
+      iFrame.
+      
+      (* iDestruct (storev_interp_mono with "HVr1") as "Hr1Mono"; eauto. *)
+      iDestruct ((storev_P_mono _ P') with "[HVr1] [Hwcond'] [Hrcond']")
+        as "HmonoP'"; eauto.
+      eauto.
+      eauto.
+      eauto.
+      eauto.
+      eauto.
+    iDestruct (region_close_next with "[$Hr $Ha1 $Hrel' $Hstate' HmonoP']") as "Hr"; eauto.
+    { intros [g Hcontr]. specialize (H2 g). done. }
+    { apply not_elem_of_cons; split; [auto|apply not_elem_of_nil]. }
+    { iSplit.
+      iPureIntro ; clear -Hflp' Hwa; destruct p0,p'; cbn in *; try done.
+      iFrame "#".
+      destruct (writeAllowed p') eqn:Hwa'; cycle 1.
+      { destruct p0, p'; cbn in *; try congruence;  inv Hflp'. }
+      by iDestruct ("Hwcond'" with "HVstorev1") as "HP'storev".
+    }
+    iDestruct (region_open_prepare with "Hr") as "$".
+    + subst a0. iDestruct "HStoreRes" as "[-> [HStoreRes %]]".
+      rewrite insert_insert -memMap_resource_1.
+      rewrite lookup_insert in Ha0; inversion Ha0; simplify_eq.
+      iExists storev. iFrame. rewrite /wcond'.
+      rewrite decide_True.
+      2:{
+        rewrite /writeAllowed_in_r_a. eexists r1, _. inversion Hras.
+        split. eassumption.
+        destruct H1. destruct H2.
+        split;auto.
+        split;auto.
+        destruct H2.
+        apply withinBounds_le_addr in H2; auto.
+      }
+      iSplitR;[iApply "Hwcond";iFrame "#"|].
+      iDestruct (storev_interp_mono with "HVr1") as "Hr1Mono"; eauto.
+      rewrite /monotonicity_guarantees_region.
+      destruct ρ;auto.
+      { destruct (pwl pc_p'); iModIntro; iIntros (W1 W2 Hrelated) "H".
+        all:iApply "Hwcond"; iApply "Hr1Mono"; eauto; iApply "Hrcond"; iFrame.
+      }
+      { destruct (pwl pc_p'); iModIntro; iIntros (W1 W2 Hrelated) "H".
+        all:iApply "Hwcond"; iApply "Hr1Mono"; eauto; iApply "Hrcond"; iFrame.
+      }
+   Qed.
+
+   Lemma if_later {C} {eqdec: Decision C} (Q Q' : iProp Σ) : (if (decide C) then ▷ Q else Q') -∗ ▷ (if (decide C) then Q else Q').
    Proof. iIntros "H". destruct (decide C);auto. Qed.
+
+   Lemma if_later_bool (b : bool) (Q Q' : iProp Σ) : (if b then ▷ Q else Q') -∗ ▷ (if b then Q else Q').
+   Proof. iIntros "H". destruct b;auto. Qed.
+
+  Lemma allow_store_mem_later:
+    ∀ (W : WORLD) (regs : leibnizO Reg)
+      (a : Addr) (w : Word) r1 r2 (p' : Perm) (mem0 : Mem),
+    allow_store_mem W r1 r2 regs a p' w mem0 true
+    -∗ ▷ allow_store_mem W r1 r2 regs a p' w mem0 false.
+  Proof.
+    iIntros (W regs a w r1 r2 p' mem0) "HStoreMem".
+    iDestruct "HStoreMem" as (p1 g1 b1 e1 a1 storev1) "[% [% HStoreRes] ]".
+    do 6 (iApply later_exist_2; iExists _).
+    iApply later_sep_2; iSplitR; auto.
+    iApply later_sep_2; iSplitR; auto.
+    case_decide; last iFrame.
+    case_decide; last iFrame.
+    iDestruct "HStoreRes" as (p0 P w0 Hp'O Hpers) "(#Hzcond & #Hwcond & #Hrcond & -> & HStoreMem)".
+    repeat (iApply later_exist_2; iExists _).
+    repeat (iApply later_sep_2; iSplitR; auto).
+    iDestruct (if_later_bool with "Hwcond") as "Hwcond'"; eauto.
+    iDestruct (if_later_bool with "Hrcond") as "Hrcond'"; eauto.
+  Qed.
 
    Lemma store_case (W : WORLD) (regs : leibnizO Reg)
      (p p' : Perm) (g : Locality) (b e a : Addr) (w : Word)
@@ -408,6 +660,8 @@ Section fundamental.
     { iSplitR "Hmap"; auto. }
     rewrite /wcond.
     iDestruct (if_later with "Hwcond") as "Hwcond'";auto.
+    iDestruct (allow_store_mem_later with "HStoreMem") as "HStoreMem".
+
     iNext. iIntros (regs' mem' retv). iDestruct 1 as (HSpec) "[Hmem Hmap]".
 
     destruct HSpec as [* ? ? ? -> Hincr|].
@@ -424,7 +678,8 @@ Section fundamental.
 
       (* Step 4: return all the resources we had in order to close the second location
          in the region, in the cases where we need to *)
-      iDestruct (mem_map_recover_res with "HStoreMem Hreg Hinv_interp Hw Hrcond [Hwcond] Hmono Hmem")
+      iDestruct (mem_map_recover_res
+                  with "HStoreMem Hreg Hinv_interp Hw Hrcond [Hwcond] Hmono Hmem")
         as (w') "(Hr & Ha & HSVInterp & Hmono)"; eauto.
 
       iDestruct (switch_monotonicity_formulation with "Hmono") as "Hmono"; auto.
